verified/sha/sha256.i.dfy
@@ -550,8 +550,3 @@ function {:opaque} bswap32_seq(input:seq<word>) : seq<word>
     if input == [] then []
     else [bswap32(input[0])] + bswap32_seq(input[1..])
 }
-
-predicate ValidAddrs(base:int, num_words:int)
-{
-    ValidMemRange(base, base + num_words * WORDSIZE)
-}
